wip: defining PR for wait-freedom proofs

lawyer/nonblocking/pr_wfree.v
@@ -1,51 +1,177 @@
 From iris.proofmode Require Import tactics.
 From trillium.traces Require Import inftraces trace_lookup exec_traces trace_len. 
-From trillium.program_logic Require Import execution_model weakestpre adequacy simulation_adequacy_em_cond. 
-From trillium.prelude Require Import classical.
-From fairness Require Import fairness.
+From trillium.program_logic Require Import execution_model weakestpre adequacy_utils adequacy_cond simulation_adequacy_em_cond. 
+From fairness Require Import fairness locales_helpers.
 From lawyer Require Import program_logic sub_action_em action_model.
-From lawyer.examples Require Import orders_lib obls_tactics.
-From lawyer.obligations Require Import obligations_resources obligations_logic env_helpers obligations_adequacy obligations_model obligations_em obligations_am obls_termination.
+(* From lawyer.examples Require Import orders_lib obls_tactics. *)
+From lawyer.obligations Require Import obligations_resources obligations_logic env_helpers obligations_adequacy obligations_model obligations_em obligations_am.
 From heap_lang Require Import lang.
-From lawyer.nonblocking Require Import trace_context.
-
-Definition LoopingModel: Model :=
-  {| mstate := unit; mlabel := unit; mtrans := fun _ _ _ => True |}.
-
-(* Class LoopIrisG {Λ: language} Σ := { *)
-(*     lig_inner :: irisG Λ LoopingModel Σ *)
-(* }. *)
+From lawyer.nonblocking Require Import trace_context om_wfree_inst.
 
 
-  (* Program Definition WptpPR {Σ} {Hinv : @IEMGS _ _ LG_EM EM Σ} *)
-  (*   (iG := IEM_irisG LG_EM EM) *)
-  (*   : ProgressResource state_interp (fun _ _ => ⌜ True ⌝%I) fork_post C := *)
-  (*   {| pr_pr := (fun s etr Φs => wptp s (trace_last etr).1 Φs) |}.  *)
-  (* Next Obligation.  *)
-  (*   intros. apply wptp_of_val_post. *)
-  (* Qed. *)
-  (* Next Obligation.  *)
-  (*   clear R FILTER_PCL C_DEC. *)
-  (*   intros. rewrite H0. *)
-  (*   iIntros "? WPS". *)
-  (*   iMod (wptp_not_stuck_same _ _ _ _ [] with "[$] [WPS]") as "(?&?&%NS)".  *)
-  (*   3: by iFrame. *)
-  (*   { eauto. } *)
-  (*   { erewrite app_nil_l, app_nil_r. *)
-  (*     erewrite <- surjective_pairing. apply trace_ends_in_last. } *)
-  (*   iModIntro. iFrame. *)
-  (*   iPureIntro. intros. subst. rewrite -H0. *)
-  (*   eapply NS; eauto. *)
-  (*   apply last_eq_trace_ends_in in H0. rewrite H0. simpl. set_solver. *)
-  (* Qed. *)
-  (* Final Obligation.  *)
-  (*   intros. *)
-  (*   iIntros "?? _ ? _". (** for usual wptp with the same TI, trivial trace invariant and any trace condition don't matter *) *)
-  (*   iMod (take_step with "[$] [$] [$]") as "X". *)
-  (*   1, 2: by eauto. *)
-  (*   { by rewrite H0. } *)
-  (*   iModIntro. iApply (step_fupdN_mono with "[$]"). *)
-  (*   iIntros "X". iMod "X" as "(?&?)". iModIntro. iFrame.  *)
-  (*   setoid_rewrite bi.True_sep'. by rewrite H0. *)
-  (* Qed. *)
+Close Scope Z.
 
+
+Section Pwp.
+
+  Definition LoopingModel: Model :=
+    {| mstate := unit; mlabel := unit; mtrans := fun _ _ _ => True |}.
+
+  (* Class LoopIrisG {Λ: language} Σ := { *)
+  (*   lig_inner :: irisG Λ LoopingModel Σ *)
+  (* }. *)
+
+  (* Definition pwp {Λ: language} {Σ: gFunctors} := @wp Λ (iProp Σ) LoopingModel. *)
+  (* Definition pwp := @wp (A := LoopingModel). *)
+  (* Definition pwp {Λ: language} {PROP} := @wp Λ PROP LoopingModel. *)
+  (* Global Arguments pwp {_ _ _}.  wp *)
+  Definition pwp `{!irisG Λ LoopingModel Σ} :=
+    @wp Λ (iProp Σ) stuckness _. 
+
+End Pwp. 
+
+
+Section WaitFreePR.
+
+  Let OP := LocaleOP (OPRE := OPP_WF) (Locale := locale heap_lang). 
+  Existing Instance OP.
+  Let OM := ObligationsModel.
+
+  Let M := AM2M ObligationsAM.
+  Let ASEM := ObligationsASEM.
+  Let EM := TopAM_EM ASEM (fun {Σ} {aGS: asem_GS Σ} τ _ => obls τ ∅ (oGS := aGS)).
+
+  Context (ic: @trace_ctx heap_lang).
+  Let ii := tctx_index ic.
+  Let Ki := tctx_ctx ic.
+  Let τi := tctx_tid ic.
+
+  Context (m: val).
+  Context (F: nat). (** amount of fuel required for the call (currently at d0) *)
+
+  Definition no_extra_obls (_: cfg heap_lang) (δ: mstate M) :=
+    forall τ', default ∅ (ps_obls δ !! τ') ≠ ∅ -> τ' = τi.
+
+  Definition obls_sim_rel_wfree extr omtr :=
+    obls_sim_rel extr omtr /\ no_extra_obls (trace_last extr) (trace_last omtr).
+
+  Definition wfree_trace_inv `{Hinv : @IEMGS _ _ HeapLangEM EM Σ}
+    (extr: execution_trace heap_lang) (omtr: auxiliary_trace M): iProp Σ :=
+    ⌜ no_extra_obls (trace_last extr) (trace_last omtr) ⌝.
+
+  Definition fits_inf_call: execution_trace heap_lang → Prop.
+  Admitted.
+
+  Definition phys_SI {Σ} {Hinv : @IEMGS _ _ HeapLangEM EM Σ}
+    (etr: execution_trace heap_lang) (_: auxiliary_trace LoopingModel): iProp Σ :=
+    lgem_si (trace_last etr).2 (lgem_GS0 := (iem_phys HeapLangEM EM)).
+
+  (* TODO: move *)
+  Definition wptp_from_gen {Σ: gFunctors}
+    (W: expr -> locale heap_lang -> (val → iPropI Σ) -> iProp Σ)
+    (t0 t: list expr) (Φs : list (val → iPropI Σ)) :=
+    ([∗ list] tp1_e;Φ ∈ (prefixes_from t0 t);Φs,
+       W tp1_e.2 (locale_of tp1_e.1 tp1_e.2) Φ)%I.
+
+  Definition wptp_gen {Σ} W t Φs := (@wptp_from_gen Σ W [] t Φs).
+
+  (** not making it an instance to avoid incorrect Iris instantiations *)
+  Definition iris_OM_into_Looping {Σ} (Hinv: @IEMGS _ _ HeapLangEM EM Σ):
+    irisG heap_lang LoopingModel Σ.
+  Proof using.
+    exact {| state_interp := phys_SI; fork_post := fun _ _ => (⌜ True ⌝)%I |}.
+  Defined.
+
+  (* TODO: move *)
+  Definition under_ctx (K: ectx heap_lang) (e: expr): option expr.
+  Admitted.
+
+  Lemma under_ctx_spec K e e':
+    under_ctx K e = Some e' <-> ectx_fill K e' = e.
+  Proof using. Admitted.
+
+  (* Definition empty_post {Σ: gFunctors}: val -> iProp Σ := (fun _ => ⌜ True ⌝%I).  *)
+
+  Definition wp_tc {Σ} {Hinv : @IEMGS _ _ HeapLangEM EM Σ}
+    (s: stuckness) (e: expr) (b: bool) Φ :=
+    if b then
+      let e' := default (Val #false) (under_ctx Ki e) in
+      wp s ⊤ τi e' Φ
+    else
+      let _ := iris_OM_into_Looping in
+      pwp s ⊤ τi e Φ.
+
+  Definition wptp_wfree {Σ} {Hinv : @IEMGS _ _ HeapLangEM EM Σ}
+    (s: stuckness)
+    (* (tp: list expr) *)
+    (etr: execution_trace heap_lang)
+    (Φs : list (val → iPropI Σ)):
+    iProp Σ :=
+    wptp_gen (fun e τ Φ => if decide (τi = τ) 
+                          then wp_tc s e (ii <? trace_length etr) Φ
+                          else
+                            let _ := iris_OM_into_Looping in
+                            pwp s ⊤ τ e Φ)
+      (trace_last etr).1 Φs.
+
+  Open Scope WFR_scope. 
+
+  Definition extra_fuel `{!ObligationsGS Σ} (etr: execution_trace heap_lang) :=
+    let len := trace_length etr in
+    if len <? ii then (cp_mul π0 d0 (ii - len) ∗ cp_mul π0 d0 F)%I else ⌜ True ⌝%I.
+
+  (* TODO: need to support the situation where 1/2 of τ's phase is taken out *)
+  (*      already in the starting state - use a token? *)
+  Definition cur_phases `{!ObligationsGS Σ} (etr: execution_trace heap_lang): iProp Σ :=
+    let c := trace_last etr in
+    (* ([∗ map] τ' ↦ π' ∈ delete τ (ps_phases δ), th_phase_eq τ' π') ∗ *)
+    ([∗ set] τ ∈ locales_of_cfg c ∖ {[ τi ]}, ∃ π, th_phase_eq τ π) ∗
+    let ph_res := let q := if (trace_length etr <? ii) then 1%Qp else (/2)%Qp in
+                  (∃ π, th_phase_frag τi π q)%I in
+    ⌜ τi ∈ locales_of_cfg c ⌝ → ph_res.
+
+  Definition cur_obls_sigs `{!ObligationsGS Σ} (etr: execution_trace heap_lang): iProp Σ :=
+    let c := trace_last etr in
+    ([∗ set] τ ∈ locales_of_cfg c ∖ {[ τi ]}, obls τ ∅) ∗
+    if decide (τi ∈ locales_of_cfg c)
+    then (∃ s, obls τi {[ s ]} ∗ sgn s l0 (Some false) ∗ ep s π0 d0)%I
+    else cp π0 d1.
+
+  (* Lemma foo {Σ} {Hinv : @IEMGS _ _ HeapLangEM EM Σ}: ObligationsGS Σ. *)
+  (*   apply Hinv. *)
+  (*   Show Proof.  *)
+  (*   apply _.  *)
+  
+  Definition pr_pr_wfree {Σ} {Hinv : @IEMGS _ _ HeapLangEM EM Σ}
+    (s: stuckness) (etr: execution_trace heap_lang) (Φs: list (val → iProp Σ)): iProp Σ :=
+    let oGS: ObligationsGS Σ := @iem_fairnessGS _ _ _ _ _ Hinv in
+    wptp_wfree s etr Φs ∗ extra_fuel etr ∗ cur_phases etr ∗ cur_obls_sigs etr. 
+
+(*   Definition obls_wfree_ti `{!ObligationsGS Σ} *)
+(*     (etr: execution_trace Λ) (omtr: auxiliary_trace OM): iProp Σ := *)
+(*     obls_ti etr omtr ∗ extra_fuel omtr ∗ cur_phases omtr ∗ cur_obls_sigs omtr. *)
+
+  Program Definition PR_wfree {Σ} {Hinv : @IEMGS _ _ HeapLangEM EM Σ}:
+    @ProgressResource heap_lang M Σ (@iem_invGS _ _ _ _ _ Hinv)
+      state_interp wfree_trace_inv fork_post fits_inf_call :=
+    {| pr_pr := pr_pr_wfree |}.
+  Next Obligation.
+    intros.
+    rewrite /pr_pr_wfree.
+    iIntros "(WPS & CPS & PH & OB)".
+    iAssert (|~~| (Ps ∗ (Ps -∗ wptp_wfree s ex Φs)))%I with "[WPS]" as "CLOS".
+    2: { iMod "CLOS". iModIntro. by iFrame. }
+    rewrite /wptp_wfree.
+    iDestruct (big_sepL2_length with "[$]") as "%LENS".
+    rewrite adequacy_utils.prefixes_from_length in LENS.
+    (* split thread pool into three parts, 
+       "frame" the outer two using wptp_of_val_post,
+       prove the remaining wp/pwp part for τi *)
+    admit.
+  Admitted.
+  Next Obligation.
+  Admitted. 
+  Final Obligation.
+  Admitted. 
+  
+End WaitFreePR.
