lawyer/nonblocking/obligations_wfree_em.v
@@ -1,85 +1,67 @@
-From iris.proofmode Require Import tactics.
-From trillium.traces Require Import inftraces trace_lookup exec_traces trace_len. 
-From trillium.program_logic Require Import execution_model weakestpre adequacy. 
-From fairness Require Import fairness.
-From lawyer.examples Require Import orders_lib.
-From lawyer.obligations Require Import obligations_resources obligations_model obligations_em.
+(* From iris.proofmode Require Import tactics. *)
+(* From trillium.traces Require Import inftraces exec_traces trace_len.  *)
+(* From trillium.program_logic Require Import execution_model weakestpre adequacy.  *)
+(* From fairness Require Import fairness. *)
+(* From lawyer.examples Require Import orders_lib. *)
+(* From lawyer.obligations Require Import obligations_resources obligations_model obligations_em. *)
 
 
-Section TraceContext.
-  Context `{EqDecision (locale Λ)}.
+(* Section ObligationsWaitFreeEM. *)
+(*   Context `{Countable (locale Λ)}. *)
 
-  Record trace_ctx := TraceCtx {
-    tctx_index: nat;
-    tctx_tid: locale Λ;
-    tctx_ctx: ectx Λ;
-  }.
+(*   Context (ic: @trace_ctx Λ). (** location of the infinite call *) *)
+
+
+
+(*   Definition obls_wfree_is_init_st (σ: cfg Λ) (δ: mstate OM): Prop. *)
+(*   Admitted. *)
+(*     (* obls_is_init_st σ δ /\ *) *)
+    
+(*   Lemma obls_wfree_resources_init Σ {PRE: ObligationsPreGS Σ}: *)
+(*     ∀ s1 σ p (INIT: obls_is_init_st σ s1), *)
+(*         ⊢ |==> ∃ eGS: ObligationsGS Σ, obls_init_resource s1 p ∗ obls_wfree_ti {tr[ σ ]} {tr[ s1 ]}. *)
+(*   Proof using. *)
+(*     clear H1 H0 H.  *)
+(*     simpl. intros δ σ ? INIT. iStartProof. *)
+(*     iMod (own_alloc (● (cps_repr $ ps_cps  δ) ⋅ ◯ _)) as (?) "[CPa CPf]". *)
+(*     { by apply auth_both_valid_2. } *)
+(*     iMod (own_alloc (● (sig_map_repr (ps_sigs δ)) ⋅ ◯ _)) as (?) "[SIGSa SIGSf]". *)
+(*     { apply auth_both_valid_2; [| reflexivity]. *)
+(*       rewrite /sig_map_repr. *)
+(*       intros s. destruct lookup eqn:L; [| done]. *)
+(*       apply lookup_fmap_Some in L.  *)
+(*       destruct L as ([l b]&<-&?). *)
+(*       done. } *)
+(*     iMod (own_alloc (● (obls_map_repr $ ps_obls δ) ⋅ ◯ _)) as (?) "[OBLSa OBLSf]".  *)
+(*     { apply auth_both_valid_discrete. split; [reflexivity| ]. *)
+(*       intros τ. rewrite lookup_fmap.  *)
+(*       by destruct lookup. } *)
+(*     iMod (own_alloc (● (eps_repr $ ps_eps δ) ⋅ ◯ _)) as (?) "[EPSa EPSf]".  *)
+(*     { by apply auth_both_valid_2. } *)
+
+(*     iMod (ghost_map_alloc (wrap_phase <$> ps_phases δ)) as (?) "[PHa PHf]". *)
+(*     iMod (own_alloc (●MN (ps_exc_bound δ) ⋅ mono_nat_lb _)) as (?) "[LBa LBf]". *)
+(*     { apply mono_nat_both_valid. reflexivity. } *)
+(*     iModIntro. iExists {| obls_pre := PRE; |}. *)
+(*     rewrite big_sepM_fmap. iFrame. *)
+
+(*     rewrite /cps_repr. iSplitL. *)
+(*     { by iApply cps_mset. }  *)
+
+(*     iPureIntro.  *)
+(*     red in INIT. destruct INIT as (?&?). *)
+(*     red. rewrite /threads_own_obls /dom_phases_obls. *)
+(*     erewrite om_wf_dpo; eauto. *)
+(*   Qed. *)
   
-  Context (tr: extrace Λ). 
-
-  Definition expr_under '(TraceCtx i τ K) (e: expr Λ) :=
-    exists c, tr S!! i = Some c /\ from_locale c.1 τ = Some (ectx_fill K e).
-
-End TraceContext.
-
-
-Section ObligationsWaitFreeEM.
-  Context `{Countable (locale Λ)}.
-
-  Context (ic: @trace_ctx Λ). (** location of the infinite call *)
-  Context (F: nat). (** amount of fuel required for the call (currently at d0) *)
-
-  Definition WF_SB := 1.
-
-  Instance OP_WF: ObligationsParams (bounded_nat 2) unit (locale Λ) WF_SB.
-  esplit; try by apply _.
-  - apply nat_bounded_PO.
-  - apply unit_PO.
-  Defined.
-
-  Let OM := ObligationsModel.
-  Notation "'Degree'" := (bounded_nat 2). 
-  Notation "'Level'" := (unit).
-
-  Let d0: Degree := ith_bn 2 0 ltac:(lia).
-  Let d1: Degree := ith_bn 2 1 ltac:(lia).
-  Let l0: Level := tt.
-
-  Definition extra_fuel `{!ObligationsGS Σ} (omtr: auxiliary_trace OM) :=
-    let len := trace_length omtr in
-    let i := tctx_index ic in
-    if i <? len then (cp_mul π0 d0 (len - i) ∗ cp_mul π0 d0 F)%I else ⌜ True ⌝%I.
-
-  Definition cur_phases `{!ObligationsGS Σ} (omtr: auxiliary_trace OM): iProp Σ :=
-    let δ := trace_last omtr in
-    let τ := tctx_tid ic in
-    ([∗ map] τ' ↦ π' ∈ delete τ (ps_phases δ), th_phase_eq τ' π') ∗
-    let ph_res π := let q := if (tctx_index ic <? trace_length omtr) 
-                             then 1%Qp else (/2)%Qp
-                    in th_phase_frag τ π q in
-    from_option ph_res ⌜ True ⌝%I (ps_phases δ !! τ).
-
-  Definition cur_obls_sigs `{!ObligationsGS Σ} (omtr: auxiliary_trace OM): iProp Σ :=
-    let δ := trace_last omtr in
-    let τ := tctx_tid ic in
-    ([∗ set] τ' ∈ dom (ps_obls δ) ∖ {[ τ ]}, obls τ' ∅) ∗
-    if decide (τ ∈ dom (ps_obls δ))
-    then (∃ s, obls τ {[ s ]} ∗ sgn s l0 (Some false) ∗ ep s π0 d0)%I
-    else cp π0 d1. 
-
-  Definition obls_wfree_ti `{!ObligationsGS Σ}
-    (etr: execution_trace Λ) (omtr: auxiliary_trace OM): iProp Σ :=
-    obls_ti etr omtr ∗ extra_fuel omtr ∗ cur_phases omtr ∗ cur_obls_sigs omtr.
-
-  foobar. 
-  Definition ObligationsEM: ExecutionModel Λ OM :=
-    {| 
-      em_Σ := obls_Σ;
-      em_valid_evolution_step := obls_valid_evolution_step;
-      em_thread_post Σ `{!ObligationsGS Σ} :=
-        fun τ _ => (obls τ ∅)%I;
-      em_initialization := obls_resources_init;
-    |}.
+(*   Definition ObligationsEM: ExecutionModel Λ OM := *)
+(*     {|  *)
+(*       em_Σ := obls_Σ; *)
+(*       em_valid_evolution_step := obls_valid_evolution_step; *)
+(*       em_thread_post Σ `{!ObligationsGS Σ} := *)
+(*         fun τ _ => (obls τ ∅)%I; *)
+(*       em_initialization := obls_resources_init; *)
+(*     |}. *)
 
 
-End ObligationsWaitFreeEM.
+(* End ObligationsWaitFreeEM. *)
